RegexCorrectness/Regex/Matches.lean
@@ -7,8 +7,9 @@ open String (Pos)
 
 namespace Regex.Matches
 
-def Spec {re : Regex} (s : re.IsSearchRegex) (positions : Pos × Pos) : Prop :=
+def Spec {re : Regex} (s : re.IsSearchRegex) (haystack : String) (positions : Pos × Pos) : Prop :=
   ∃ l m r groups,
+    haystack = ⟨l ++ m ++ r⟩ ∧
     s.expr.Captures ⟨l, [], m ++ r⟩ ⟨l, m.reverse, r⟩ groups ∧
     positions.1 = ⟨String.utf8Len l⟩ ∧
     positions.2 = ⟨String.utf8Len l + String.utf8Len m⟩
@@ -18,7 +19,7 @@ def Valid (self : Matches) : Prop :=
 
 theorem captures_of_next?_some {self self' : Matches} {positions} (h : self.next? = .some (positions, self'))
   (v : self.Valid) :
-  self'.Valid ∧ Spec v.1 positions := by
+  self'.Valid ∧ Spec v.1 self.haystack positions := by
   unfold next? at h
   split at h
   next lt =>
@@ -28,6 +29,7 @@ theorem captures_of_next?_some {self self' : Matches} {positions} (h : self.next
     | some matched =>
       simp at h
       have ⟨l, m, r, groups, eqstring, c, eq₁, eq₂⟩ := v.1.searchNext_some h' v.2
+      simp at eqstring
       split at h
       next =>
         simp at h
@@ -35,17 +37,29 @@ theorem captures_of_next?_some {self self' : Matches} {positions} (h : self.next
         have vp : Pos.Valid self.haystack matched.2 := by
           simp [eq₂]
           refine ⟨l ++ m, r, ?_, by simp⟩
-          simp at eqstring
           simp [eqstring]
-        exact ⟨⟨v.1, vp⟩, l, m, r, groups, c, eq₁, eq₂⟩
+        exact ⟨⟨v.1, vp⟩, l, m, r, groups, by simp [eqstring], c, eq₁, eq₂⟩
       next =>
         simp at h
         simp [←h, Valid]
-        exact ⟨⟨v.1, String.valid_next v.2 lt⟩, l, m, r, groups, c, eq₁, eq₂⟩
+        exact ⟨⟨v.1, String.valid_next v.2 lt⟩, l, m, r, groups, by simp [eqstring], c, eq₁, eq₂⟩
   next => simp at h
 
 theorem regex_eq_of_next?_some {self self' : Matches} {positions} (h : self.next? = .some (positions, self')) :
   self'.regex = self.regex := by
+  unfold next? at h
+  split at h
+  next =>
+    set matched := VM.searchNext self.regex.nfa self.regex.wf ⟨self.haystack, self.currentPos⟩
+    match h' : matched with
+    | none => simp at h
+    | some matched =>
+      simp at h
+      split at h <;> simp at h <;> simp [←h]
+  next => simp at h
+
+theorem haystack_eq_of_next?_some {self self' : Matches} {positions} (h : self.next? = .some (positions, self')) :
+  self'.haystack = self.haystack := by
   unfold next? at h
   split at h
   next =>
