RegexCorrectness/Regex/Utilities.lean
@@ -12,25 +12,26 @@ variable {re : Regex} {haystack : String}
 
 theorem captures_of_find_some {positions} (h : re.find haystack = .some positions)
   (s : re.IsSearchRegex) :
-  Matches.Spec s positions := by
+  Matches.Spec s haystack positions := by
   simp [Regex.find] at h
   have ⟨_, h⟩ := h
   have v := Captures.valid_captures haystack s
   exact (Matches.captures_of_next?_some h v).2
 
 theorem captures_of_mem_findAll.go {m : Matches} {accum : Array (Pos × Pos)}
-  (v : m.Valid) (inv : ∀ positions ∈ accum, Matches.Spec v.1 positions) :
-  ∀ positions ∈ findAll.go m accum, Matches.Spec v.1 positions := by
+  (v : m.Valid) (inv : ∀ positions ∈ accum, Matches.Spec v.1 m.haystack positions) :
+  ∀ positions ∈ findAll.go m accum, Matches.Spec v.1 m.haystack positions := by
   induction m, accum using findAll.go.induct with
   | case1 m accum positions m' next_some? ih =>
     -- next match is found
     rw [findAll.go, next_some?]
     simp
     have regex_eq := Matches.regex_eq_of_next?_some next_some?
-    simp [regex_eq] at ih
+    have haystack_eq := Matches.haystack_eq_of_next?_some next_some?
+    simp [regex_eq, haystack_eq] at ih
 
     have ⟨v', spec⟩ := Matches.captures_of_next?_some next_some? v
-    have inv' (p₁ p₂ : Pos) (mem : (p₁, p₂) ∈ accum.push positions) : Matches.Spec v.1 (p₁, p₂) := by
+    have inv' (p₁ p₂ : Pos) (mem : (p₁, p₂) ∈ accum.push positions) : Matches.Spec v.1 m.haystack (p₁, p₂) := by
       simp [Array.push_eq_append_singleton] at mem
       cases mem with
       | inl mem => exact inv (p₁, p₂) mem
@@ -44,32 +45,33 @@ theorem captures_of_mem_findAll.go {m : Matches} {accum : Array (Pos × Pos)}
 
 theorem captures_of_mem_findAll {positions} (mem : positions ∈ re.findAll haystack)
   (s : re.IsSearchRegex) :
-  Matches.Spec s positions := by
+  Matches.Spec s haystack positions := by
   simp [Regex.findAll] at mem
   have v := Matches.vaild_matches haystack s
   exact captures_of_mem_findAll.go v (by simp) positions mem
 
 theorem captures_of_capture_some {captured} (h : re.capture haystack = .some captured)
   (s : re.IsSearchRegex) :
-  captured.Spec s := by
+  captured.Spec s haystack := by
   simp [Regex.capture] at h
   have ⟨_, h⟩ := h
   have v := Captures.valid_captures haystack s
   exact (Captures.captures_of_next?_some h v).2
 
 theorem captures_of_mem_captureAll.go {captures : Captures} {accum : Array CapturedGroups}
-  (v : captures.Valid) (inv : ∀ captured ∈ accum, captured.Spec v.1) :
-  ∀ captured ∈ captureAll.go captures accum, captured.Spec v.1 := by
+  (v : captures.Valid) (inv : ∀ captured ∈ accum, captured.Spec v.1 captures.haystack) :
+  ∀ captured ∈ captureAll.go captures accum, captured.Spec v.1 captures.haystack := by
   induction captures, accum using captureAll.go.induct with
   | case1 captures accum groups captures' next?_some ih =>
     -- next capture is found
     rw [captureAll.go, next?_some]
     simp
     have regex_eq := Captures.regex_eq_of_next?_some next?_some
-    simp [regex_eq] at ih
+    have haystack_eq := Captures.haystack_eq_of_next?_some next?_some
+    simp [regex_eq, haystack_eq] at ih
 
     have ⟨v', spec⟩ := Captures.captures_of_next?_some next?_some v
-    have inv' (captured : CapturedGroups) (mem : captured ∈ accum.push groups) : captured.Spec v.1 := by
+    have inv' (captured : CapturedGroups) (mem : captured ∈ accum.push groups) : captured.Spec v.1 captures.haystack := by
       simp [Array.push_eq_append_singleton] at mem
       cases mem with
       | inl mem => exact inv captured mem
@@ -83,7 +85,7 @@ theorem captures_of_mem_captureAll.go {captures : Captures} {accum : Array Captu
 
 theorem captures_of_mem_captureAll {captured} (mem : captured ∈ re.captureAll haystack)
   (s : re.IsSearchRegex) :
-  captured.Spec s := by
+  captured.Spec s haystack := by
   simp [Regex.captureAll] at mem
   have v := Captures.valid_captures haystack s
   exact captures_of_mem_captureAll.go v (by simp) captured mem
